small cleanups

Carleson/ForestOperator/Forests.lean
@@ -51,37 +51,31 @@ lemma correlation_separated_trees (hu₁ : u₁ ∈ t) (hu₂ : u₂ ∈ t) (hu 
 /-! ## Section 7.7 -/
 
 def rowDecomp_zornset (t : Forest X n) (s : Set (𝔓 X)) :=
-  { x : Set (𝔓 X)
-    | x ⊆ s
-    ∧ x.PairwiseDisjoint t
-    ∧ ∀ u ∈ x, Maximal (· ∈ ((fun x => 𝓘 x : 𝔓 X → Set X) '' s)) (𝓘 u : Set X) }
+  { x : Set (𝔓 X) | x ⊆ s} ∩ {x : Set (𝔓 X) | x.PairwiseDisjoint t} ∩
+    {x : Set (𝔓 X) | x ⊆ {u | Maximal (· ∈ ((fun x => 𝓘 x : 𝔓 X → Set X) '' s)) (𝓘 u : Set X)}}
 
 lemma mem_rowDecomp_zornset_iff (t : Forest X n) (s s' : Set (𝔓 X)) :
     s' ∈ rowDecomp_zornset t s ↔ (s' ⊆ s ∧ s'.PairwiseDisjoint t ∧
       ∀ u ∈ s', Maximal (· ∈ (fun x => 𝓘 x : 𝔓 X → Set X) '' s) (𝓘 u : Set X)) := by
-  rw [rowDecomp_zornset,mem_setOf]
+  rw [rowDecomp_zornset,mem_inter_iff,mem_inter_iff,mem_setOf,mem_setOf,mem_setOf,and_assoc]
+  nth_rw 2 [subset_def]
+  simp_rw [mem_setOf]
 
-lemma rowDecomp_zornset_chain_Union_bound (s' : Set (𝔓 X)) (c : Set (Set (𝔓 X))) (hc : c ⊆ t.rowDecomp_zornset s')
+lemma rowDecomp_zornset_chain_Union_bound (s' : Set (𝔓 X)) {c : Set (Set (𝔓 X))} (hc : c ⊆ t.rowDecomp_zornset s')
     (hc_chain : IsChain (· ⊆ ·) c) :
     (⋃ s ∈ c,s) ∈ t.rowDecomp_zornset s' ∧ ∀ s ∈ c, s ⊆ ⋃ s'' ∈ c, s'' := by
-  have hc' := fun a (h : a ∈ c) => hc h
-  simp_rw [mem_rowDecomp_zornset_iff] at hc ⊢
-  repeat' constructor
-  · simp_rw [iUnion_subset_iff]
-    intro s hs
-    specialize hc' s hs
-    exact hc'.left
-  · apply hc_chain.pairwiseDisjoint_iUnion₂
-    exact fun s hs => (hc' s hs).right.left
-  · simp only [mem_iUnion, exists_prop, forall_exists_index, and_imp]
-    exact fun u s hs => (hc' s hs).right.right u
+  simp_rw [rowDecomp_zornset,subset_inter_iff] at hc ⊢
+  obtain ⟨⟨hc₁,hc₂⟩,hc₃⟩ := hc
+  simp_rw [mem_inter_iff,mem_setOf]
+  repeat constructor
+  · exact iUnion₂_subset_iff.mpr hc₁
+  · exact hc_chain.pairwiseDisjoint_iUnion₂ _ _ hc₂
+  · exact iUnion₂_subset_iff.mpr hc₃
   · exact fun s a_1 ↦ subset_iUnion₂_of_subset s a_1 fun ⦃a_2⦄ a ↦ a
 
 def rowDecomp_𝔘 (t : Forest X n) (j : ℕ) : Set (𝔓 X) :=
-  (zorn_subset
-  (rowDecomp_zornset t (t \ ⋃ i < j, rowDecomp_𝔘 t i))
-  (fun c hc hc_chain => ⟨⋃ s ∈ c, s, rowDecomp_zornset_chain_Union_bound _ c hc hc_chain⟩
-  )).choose
+  (zorn_subset (rowDecomp_zornset t (t \ ⋃ i < j, rowDecomp_𝔘 t i))
+  (fun _ hc => Exists.intro _ ∘ rowDecomp_zornset_chain_Union_bound _ hc)).choose
 
 lemma rowDecomp_𝔘_def (t : Forest X n) (j : ℕ) :
     Maximal (fun x ↦ x ∈ rowDecomp_zornset t (t \ ⋃ i < j, rowDecomp_𝔘 t i)) (rowDecomp_𝔘 t j) := by
@@ -94,23 +88,24 @@ lemma rowDecomp_𝔘_mem_zornset (t : Forest X n) (j : ℕ) :
 
 lemma rowDecomp_𝔘_subset (t : Forest X n) (j : ℕ) :
     t.rowDecomp_𝔘 j ⊆ t \ ⋃ i < j, rowDecomp_𝔘 t i := by
-  have := (rowDecomp_𝔘_def t j).prop
+  have := rowDecomp_𝔘_mem_zornset t j
   rw [mem_rowDecomp_zornset_iff] at this
   exact this.left
 
 lemma rowDecomp_𝔘_pairwiseDisjoint (t : Forest X n) (j : ℕ) :
     (t.rowDecomp_𝔘 j).PairwiseDisjoint t := by
-  have := (rowDecomp_𝔘_def t j).prop
+  have := rowDecomp_𝔘_mem_zornset t j
   rw [mem_rowDecomp_zornset_iff] at this
   exact this.right.left
 
+-- seems unused.
 lemma mem_rowDecomp_𝔘_maximal (t : Forest X n) (j : ℕ) :
     ∀ x ∈ (t.rowDecomp_𝔘 j), Maximal (· ∈ (fun x => 𝓘 x : 𝔓 X → Set X) '' (t \ ⋃ i < j, rowDecomp_𝔘 t i)) (𝓘 x : Set X) := by
-  have := (rowDecomp_𝔘_def t j).prop
+  have := rowDecomp_𝔘_mem_zornset t j
   rw [mem_rowDecomp_zornset_iff] at this
   exact this.right.right
 
--- maybe not important?
+-- maybe not important? not used, instead `mem_of_prop_insert` is used
 lemma rowDecomp_𝔘_maximal (t : Forest X n) (j : ℕ) :
     ∀ s ∈ rowDecomp_zornset t (t \ ⋃ i < j, rowDecomp_𝔘 t i),
     rowDecomp_𝔘 t j ⊆ s → s ⊆ rowDecomp_𝔘 t j :=
@@ -126,7 +121,6 @@ lemma rowDecomp_𝔘_stackSize_le' (t : Forest X n) (j : ℕ) :
   · exact stackSize_mono (rowDecomp_𝔘_subset_tree t j)
   · exact t.stackSize_le'
 
--- #print Row
 /-- The row-decomposition of a tree, defined in the proof of Lemma 7.7.1.
 The indexing is off-by-one compared to the blueprint. -/
 def rowDecomp (t : Forest X n) (j : ℕ) : Row X n where
@@ -145,11 +139,24 @@ def rowDecomp (t : Forest X n) (j : ℕ) : Row X n where
 lemma rowDecomp_𝔘_eq (t : Forest X n) (j : ℕ) :
   (t.rowDecomp j).𝔘 = rowDecomp_𝔘 t j := rfl
 
+-- for mathlib, maybe? if so, maybe we should also add the `Finite` and `Finset` versions?
+-- for reference, loogle for 'Maximal, "exists_le_maximal"'
 lemma Set.Finite.exists_maximal_and_mem {α : Type*} {s : Set (Set α)} (hs : s.Finite)
     {b : Set α} (hb : b ∈ s) {x : α} (hx : x ∈ b) : ∃ m, Maximal (· ∈ s) m ∧ x ∈ m :=
-  (hs.inter_of_left _ |>.exists_le_maximal (s := s ∩ {y' | x ∈ y'}) ⟨hb,hx⟩).elim
-    fun m ⟨_,hm⟩ =>
-      ⟨m,⟨⟨hm.prop.left,fun _ hm' hle => hm.le_of_ge ⟨hm',hle hm.prop.right⟩ hle⟩,hm.prop.right⟩⟩
+  (hs.inter_of_left _ |>.exists_le_maximal (s := s ∩ {y' | x ∈ y'}) ⟨hb,hx⟩).imp
+    fun _ ⟨_,hm⟩ =>
+      ⟨⟨hm.prop.left,fun _ hm' hle => hm.le_of_ge ⟨hm',hle hm.prop.right⟩ hle⟩,hm.prop.right⟩
+
+lemma stackSize_remainder_ge_one_of_exists (t : Forest X n) (j : ℕ) (x:X)
+    (this : ∃ 𝔲' ∈ (t.rowDecomp j).𝔘, x ∈ (𝓘 𝔲' : Set _)) :
+    1 ≤ stackSize ((t \ ⋃ i < j, t.rowDecomp i) ∩ t.rowDecomp j: Set _) x := by
+  obtain ⟨𝔲',h𝔲'⟩ := this
+  dsimp [stackSize]
+  rw [← Finset.sum_erase_add _ (a := 𝔲')]
+  · rw [indicator_apply,if_pos h𝔲'.right,Pi.one_apply]
+    simp only [le_add_iff_nonneg_left, zero_le]
+  simp only [mem_inter_iff, Finset.mem_filter, Finset.mem_univ, true_and]
+  exact ⟨t.rowDecomp_𝔘_subset j h𝔲'.left,h𝔲'.left⟩
 
 lemma remainder_stackSize_le (t : Forest X n) (j : ℕ) :
   ∀ x:X, stackSize (t \ ⋃ i < j, t.rowDecomp i : Set _) x ≤ 2 ^ n - j := by
@@ -168,17 +175,7 @@ lemma remainder_stackSize_le (t : Forest X n) (j : ℕ) :
         obtain ⟨𝔲,h𝔲⟩ := h
         simp only [biUnion_lt_succ, ← diff_diff] at h𝔲 ⊢
         rw [stackSize_sdiff_eq,← Nat.sub_sub]
-        gcongr
-        dsimp [stackSize]
-        suffices ∃ 𝔲' ∈ (t.rowDecomp j).𝔘, x ∈ (𝓘 𝔲' : Set _) by
-          obtain ⟨𝔲',h𝔲'⟩ := this
-          rw [← Finset.sum_erase_add _ (a := 𝔲')]
-          simp only [exists_prop, not_exists, not_and, ge_iff_le]
-          rw [indicator_apply,if_pos h𝔲'.right,Pi.one_apply]
-          simp only [le_add_iff_nonneg_left, zero_le]
-          simp only [Finset.mem_filter, Finset.mem_univ,
-            true_and,mem_inter_iff]
-          exact ⟨t.rowDecomp_𝔘_subset j h𝔲'.left,h𝔲'.left⟩
+        apply tsub_le_tsub hinduct (stackSize_remainder_ge_one_of_exists t j x _)
         rw [mem_diff] at h𝔲
         apply this.elim
         intro _ ⟨hmax,hz⟩
